examples/rv/RVCoreProperties.v
@@ -5,8 +5,9 @@ Require Import Koika.Frontend Koika.Logs Koika.Std
         Koika.ProgramTactics.
 (* Require Import Koika.SimpleTypedSemantics. *)
 Require Import UntypedSemantics.
+Require Import UntypedIndSemantics.
 Require Import BitsToLists.
-
+Require Import Coq.Program.Equality.
 (* Require Import Koika.IndTypedSemantics. *)
 
 Ltac destr_in H :=
@@ -127,26 +128,26 @@ Module StackProofs.
              (r: env_t REnv (fun _ => val))
       (sigma : RV32I.ext_fn_t -> val -> val)
   :=
-  UntypedSemantics.interp_cycle r sigma rv_urules rv_schedule.
+  UntypedSemantics.interp_cycle rv_urules r sigma rv_schedule.
 
-  Lemma extract_success_rewrite:
-    forall {S F: Type} (res1 res2: result S F) pr1 pr2,
-    res1 = res2 -> extract_success res1 pr1 = extract_success res2 pr2.
-  Proof.
-    intros. subst.
-    refine (
-      match pr1, pr2 with
-      | eq_refl _, eq_refl _ => _
-      end
-    ).
-    destruct res2; congruence.
-  Qed.
+  (* Lemma extract_success_rewrite: *)
+  (*   forall {S F: Type} (res1 res2: result S F) pr1 pr2, *)
+  (*   res1 = res2 -> extract_success res1 pr1 = extract_success res2 pr2. *)
+  (* Proof. *)
+  (*   intros. subst. *)
+  (*   refine ( *)
+  (*     match pr1, pr2 with *)
+  (*     | eq_refl _, eq_refl _ => _ *)
+  (*     end *)
+  (*   ). *)
+  (*   destruct res2; congruence. *)
+  (* Qed. *)
 
-  Lemma success_inj:
-    forall {S F: Type} (x y: S), Success x = @Success S F y -> x = y.
-  Proof.
-    intros S F x y H. inv H; auto.
-  Qed.
+  (* Lemma success_inj: *)
+  (*   forall {S F: Type} (x y: S), Success x = @Success S F y -> x = y. *)
+  (* Proof. *)
+  (*   intros S F x y H. inv H; auto. *)
+  (* Qed. *)
 
   (* Lemma cast_action'_eq: *)
   (*   forall (pos_t fn_name_t var_t reg_t ext_fn_t : Type) (R : reg_t -> type) *)
@@ -179,450 +180,68 @@ Module StackProofs.
   (* Qed. *)
 
 
-  Definition fold_desugar:
-    forall reg_t' ext_fn_t',
-      (fix
-         desugar_action' (reg_t' ext_fn_t' : Type) (pos : unit) (fR : reg_t' -> RV32I.reg_t)
-         (fSigma : ext_fn_t' -> RV32I.ext_fn_t)
-         (a0 : uaction unit var_t fn_name_t reg_t' ext_fn_t') {struct a0} :
-         uaction unit var_t fn_name_t RV32I.reg_t RV32I.ext_fn_t :=
-         match a0 with
-         | UError err => UError err
-         | {{
-               fail@(tau)
-           }} => {{
-                     fail@(tau)
-                 }}
-         | UVar var => UVar var
-         | @UConst _ _ _ _ _ tau cst => UConst cst
-         | UAssign v ex => UAssign v (desugar_action' reg_t' ext_fn_t' pos fR fSigma ex)
-         | USeq a1 a2 =>
-           USeq (desugar_action' reg_t' ext_fn_t' pos fR fSigma a1)
-                (desugar_action' reg_t' ext_fn_t' pos fR fSigma a2)
-         | UBind v ex body0 =>
-           UBind v (desugar_action' reg_t' ext_fn_t' pos fR fSigma ex)
-                 (desugar_action' reg_t' ext_fn_t' pos fR fSigma body0)
-         | UIf cond tbranch fbranch =>
-           UIf (desugar_action' reg_t' ext_fn_t' pos fR fSigma cond)
-               (desugar_action' reg_t' ext_fn_t' pos fR fSigma tbranch)
-               (desugar_action' reg_t' ext_fn_t' pos fR fSigma fbranch)
-         | URead port idx => URead port (fR idx)
-         | UWrite port idx value =>
-           UWrite port (fR idx) (desugar_action' reg_t' ext_fn_t' pos fR fSigma value)
-         | UUnop fn arg => UUnop fn (desugar_action' reg_t' ext_fn_t' pos fR fSigma arg)
-         | UBinop fn arg1 arg2 =>
-           UBinop fn (desugar_action' reg_t' ext_fn_t' pos fR fSigma arg1)
-                  (desugar_action' reg_t' ext_fn_t' pos fR fSigma arg2)
-         | UExternalCall fn arg =>
-           UExternalCall (fSigma fn) (desugar_action' reg_t' ext_fn_t' pos fR fSigma arg)
-         | UInternalCall fn args =>
-           UInternalCall
-             (map_intf_body
-                (fun a1 : uaction unit var_t fn_name_t reg_t' ext_fn_t' =>
-                   desugar_action' reg_t' ext_fn_t' pos fR fSigma a1) fn)
-             (map
-                (fun a1 : uaction unit var_t fn_name_t reg_t' ext_fn_t' =>
-                   desugar_action' reg_t' ext_fn_t' pos fR fSigma a1) args)
-         | UAPos p e => UAPos p (desugar_action' reg_t' ext_fn_t' pos fR fSigma e)
-         | USugar s => desugar reg_t' ext_fn_t' pos fR fSigma s
-         end
-             with
-               desugar (reg_t' ext_fn_t' : Type) (pos : unit) (fR : reg_t' -> RV32I.reg_t)
-               (fSigma : ext_fn_t' -> RV32I.ext_fn_t)
-               (s : usugar unit var_t fn_name_t reg_t' ext_fn_t') {struct s} :
-                 uaction unit var_t fn_name_t RV32I.reg_t RV32I.ext_fn_t :=
-           match s with
-           | UErrorInAst =>
-             UError {| epos := pos; emsg := ExplicitErrorInAst; esource := ErrSrc s |}
-           | USkip => uskip
-           | @UConstBits _ _ _ _ _ sz bs => UConst (tau:=bits_t sz) bs
-           | UConstString s0 => UConst (tau:=array_t {|array_type:=bits_t 8; array_len := length s0 |})
-                                       (array_of_bytes s0)
-           | UConstEnum sig name =>
-             match vect_index name (enum_members sig) with
-             | Some idx => UConst (tau:=enum_t sig)(vect_nth (enum_bitpatterns sig) idx)
-             | None =>
-               UError
-                 {| epos := pos; emsg := UnboundEnumMember name sig; esource := ErrSrc s |}
-             end
-           | UProgn aa =>
-             uprogn
-               (map
-                  (fun a0 : uaction unit var_t fn_name_t reg_t' ext_fn_t' =>
-                     desugar_action' reg_t' ext_fn_t' pos fR fSigma a0) aa)
-           | ULet bindings body0 =>
-             fold_right
-               (fun '(var, a0) (acc : uaction unit var_t fn_name_t RV32I.reg_t RV32I.ext_fn_t)
-                => UBind var (desugar_action' reg_t' ext_fn_t' pos fR fSigma a0) acc)
-               (desugar_action' reg_t' ext_fn_t' pos fR fSigma body0) bindings
-           | UWhen cond body0 =>
-             UIf (desugar_action' reg_t' ext_fn_t' pos fR fSigma cond)
-                 (desugar_action' reg_t' ext_fn_t' pos fR fSigma body0) {{
-                       fail@(unit_t)
-                       }}
-                 | USwitch var default branches =>
-                     uswitch (desugar_action' reg_t' ext_fn_t' pos fR fSigma var)
-                       (desugar_action' reg_t' ext_fn_t' pos fR fSigma default)
-                       (map
-                          (fun '(cond, body0) =>
-                           (desugar_action' reg_t' ext_fn_t' pos fR fSigma cond,
-                           desugar_action' reg_t' ext_fn_t' pos fR fSigma body0)) branches)
-                 | UStructInit sig fields =>
-                     ustruct_init sig
-                       (map (fun '(f, a0) => (f, desugar_action' reg_t' ext_fn_t' pos fR fSigma a0))
-                          fields)
-                 | UArrayInit tau elements =>
-                     snd
-                       (fold_left
-                          (fun '(pos0, acc) (a0 : uaction unit var_t fn_name_t reg_t' ext_fn_t') =>
-                           (S pos0,
-                           UBinop (UArray2 (USubstElement pos0)) acc
-                             (desugar_action' reg_t' ext_fn_t' pos fR fSigma a0))) elements
-                          (0,
-                          uinit
-                            (array_t {| array_type := tau; array_len := Datatypes.length elements |})))
-                 | @UCallModule _ _ _ _ _ module_reg_t module_ext_fn_t fR' fSigma' fn args =>
-                     UInternalCall
-                       (map_intf_body
-                          (fun body0 : uaction unit var_t fn_name_t module_reg_t module_ext_fn_t =>
-                           desugar_action' module_reg_t module_ext_fn_t pos
-                             (fun r : module_reg_t => fR (fR' r))
-                             (fun fn0 : module_ext_fn_t => fSigma (fSigma' fn0)) body0) fn)
-                       (map
-                          (fun a0 : uaction unit var_t fn_name_t reg_t' ext_fn_t' =>
-                           desugar_action' reg_t' ext_fn_t' pos fR fSigma a0) args)
-                 end
-                   for desugar_action') reg_t' ext_fn_t' tt =
-    desugar_action'
-      (pos_t:=unit) (var_t:=string) (fn_name_t:=string)
-      (reg_t:=RV32I.reg_t) (ext_fn_t:=RV32I.ext_fn_t)
-      (reg_t':=reg_t') (ext_fn_t' := ext_fn_t') tt.
-  Proof.
-    reflexivity.
-  Qed.
-
   Definition if_halt_eq : action (ext_fn_t:=RV32I.ext_fn_t) pos_t var_t fn_name_t RV32I.R RV32I.Sigma [] unit_t :=
     (If (Binop (PrimTyped.Eq (bits_t 1) false) (Read P0 RV32I.halt)
                (Const (tau:= bits_t 1) {| vhd := true; vtl := _vect_nil |}))
        (Fail unit_t) (Const (tau:=unit_t) _vect_nil)).
 
-  Context {reg_t_eq_dec: EqDec RV32I.reg_t}.
+  Instance reg_t_eq_dec: EqDec RV32I.reg_t.
+  Proof.
+    eapply EqDec_FiniteType.
+  Qed.
 
+  Lemma log_app_r_empty:
+    forall (REnv: Env RV32I.reg_t) (l: Log REnv), log_app l log_empty = l.
+  Proof.
+    unfold log_app. intros.
+    unfold map2.
+    etransitivity. 2: eapply create_getenv_id. apply create_funext.
+    intros. unfold log_empty.
+    rewrite getenv_create. rewrite app_nil_r. auto.
+  Qed.
+
+  Lemma get_log_cons:
+    forall (REnv: Env RV32I.reg_t) (l: Log REnv) le r1,
+      getenv REnv (log_cons r1 le l) r1 = le :: getenv REnv l r1.
+  Proof.
+    unfold log_cons. intros.
+    rewrite get_put_eq. auto.
+  Qed.
+
+  Lemma get_log_cons_other:
+    forall (REnv: Env RV32I.reg_t) (l: Log REnv) le r1 r2 (d: r1 <> r2),
+      getenv REnv (log_cons r1 le l) r2 = getenv REnv l r2.
+  Proof.
+    unfold log_cons. intros.
+    rewrite get_put_neq; auto.
+  Qed.
+
+  
   Lemma execute_overwrites_halt:
     forall REnv (r: env_t REnv _) sigma l,
       interp_rule r sigma log_empty
-                  (desugar_action tt RV32I.execute)
-                  = Some l ->
+                  RV32I.execute l ->
+      (getenv REnv r RV32I.halt <> Bits 1 [true]) ->
       log_existsb l RV32I.halt (fun k p =>
                                   match k with
                                     LogRead => false
                                   | LogWrite => true
                                   end
-                               ) = true(*  -> *)
-      (* let dbk := ContextEnv.(getenv) r (RV32I.d2e RV32I.fromDecode.data0) = dbk in *)
-      (* let dInst :=  *)
-
-        (* RV32I.isControlInst *)
-  .
+                               ) = true.
   Proof.
     intros.
-    unfold interp_rule in H.
-    destr_in H. 2: congruence.
-    repeat destr_in H. inv H.
-    unfold RV32I.execute in Heqo.
-    cbn in Heqo.
-    rewrite fold_desugar
-    unfold RV32I.execute in Heqo.
-    simpl in Heqo.
-    unfold opt_bind in Heqo. 
-    repeat destr_in Heqo. congruence. try congruence. 2: congruence.
-    unfold RV32I.tc_execute in Heqo.
-    unfold desugar_action in Heqo.
-    refine (
-      match
-        desugar_action' dummy_pos (fun r : RV32I.reg_t => r)
-        (fun fn => fn) RV32I.execute
-      with
-         x => _
-      end
-    ).
-    fold x in Heqo.
-    refine ((
-      match
-        TypeInference.tc_action RV32I.R RV32I.Sigma dummy_pos [] unit_t x
-      as r
-      return (
-        TypeInference.tc_action RV32I.R RV32I.Sigma dummy_pos [] unit_t x = r
-        -> is_success r = true -> _
-      ) with
-      | Success s => fun H1 H2 => _
-      | Failure f => fun H1 H2 => _
-      end
-    ) eq_refl eq_refl).
-    2: (simpl in H2; congruence).
-    rename Heqo into H0.
-    erewrite extract_success_rewrite in H0. 2: apply H1.
-    simpl (extract_success _ _) in H0.
-    unfold TypeInference.tc_action in H1.
-    destr_in H1. 2: congruence.
-    clear H2.
-    apply cast_action_eq in H1.
-    destruct H1 as (p & EQ). subst s.
-    revert Heqr0. simpl in x.
-    unfold eq_rect in H0.
-    destruct p.
-    unfold desugar_action' in x.
-    unfold RV32I.execute in x.
-    simpl in x.
-    unfold execALU32 in x. simpl in x.
-    unfold RV32I.fromDecode.deq in x. simpl in x.
-    unfold map_intf_body in x. vm_compute in x.
-    unfold x. clear x.
-    intro Heqr0.
-    vm_compute in Heqr0.
-    Set Printing Depth 20.
-    Set Printing All.
-    inv Heqr0.
-    apply success_inj in Heqr0.
-    subst.
-    simpl projT1 in v.
-    simpl projT2 in H0.
-
-    inversion H0.
-    apply Eqdep_dec.inj_pair2_eq_dec in H11.
-    2:{
-      apply eq_dec.
-    }
-    apply Eqdep_dec.inj_pair2_eq_dec in H7.
-    apply Eqdep_dec.inj_pair2_eq_dec in H7.
-    apply Eqdep_dec.inj_pair2_eq_dec in H8.
-    apply Eqdep_dec.inj_pair2_eq_dec in H8.
-    apply Eqdep_dec.inj_pair2_eq_dec in H8.
-    assert (var = "res"). eapply EqdepFacts.eq_sigT_fst; eauto. subst.
-    apply Eqdep_dec.inj_pair2_eq_dec in H8.
-    simpl projT1 in *.
-    apply Eqdep_dec.inj_pair2_eq_dec in H10. subst.
-    apply Eqdep_dec.inj_pair2_eq_dec in H.
-    all: try apply eq_dec. clear H0.
-    subst.
-    inv H12.
-    apply Eqdep_dec.inj_pair2_eq_dec in H.
-    apply Eqdep_dec.inj_pair2_eq_dec in H3.
-    apply Eqdep_dec.inj_pair2_eq_dec in H7.
-    apply Eqdep_dec.inj_pair2_eq_dec in H5.
-    apply Eqdep_dec.inj_pair2_eq_dec in H3. subst.
-    all: try apply eq_dec.
-    inv H9.
-    apply Eqdep_dec.inj_pair2_eq_dec in H6.
-    apply Eqdep_dec.inj_pair2_eq_dec in H11.
-    apply Eqdep_dec.inj_pair2_eq_dec in H12.
-    apply Eqdep_dec.inj_pair2_eq_dec in H1.
-    apply Eqdep_dec.inj_pair2_eq_dec in H6. subst.
-    all: try apply eq_dec.
-    inv H8.
-    apply Eqdep_dec.inj_pair2_eq_dec in H4.
-    apply Eqdep_dec.inj_pair2_eq_dec in H9.
-    apply Eqdep_dec.inj_pair2_eq_dec in H9.
-    apply Eqdep_dec.inj_pair2_eq_dec in H9.
-    apply Eqdep_dec.inj_pair2_eq_dec in H12.
-    apply Eqdep_dec.inj_pair2_eq_dec in H14. subst.
-    all: try apply eq_dec.
-
-
-    destruct (interp_action r sigma CtxEmpty log_empty log_empty RV32I.tc_end_execution) eqn:?.
-    2:{
-      Set Printing All.
-    }
-    destr_in H.
-    inv H.
-    unfold RV32I.tc_end_execution in H0.
-    unfold desugar_action in H0.
-    refine (
-      match
-        desugar_action' dummy_pos (fun r : RV32I.reg_t => r)
-        (fun fn => fn) RV32I.end_execution
-      with
-         x => _
-      end
-    ).
-    fold x in H0.
-    refine ((
-      match
-        TypeInference.tc_action RV32I.R RV32I.Sigma dummy_pos [] unit_t x
-      as r
-      return (
-        TypeInference.tc_action RV32I.R RV32I.Sigma dummy_pos [] unit_t x = r
-        -> is_success r = true -> _
-      ) with
-      | Success s => fun H1 H2 => _
-      | Failure f => fun H1 H2 => _
-      end
-    ) eq_refl eq_refl).
-    2: (simpl in H2; congruence).
-    erewrite extract_success_rewrite in H0. 2: apply H1.
-    simpl (extract_success _ _) in H0.
-    unfold TypeInference.tc_action in H1.
-    destr_in H1. 2: congruence.
-    clear H2.
-    apply cast_action_eq in H1.
-    destruct H1 as (p & EQ). subst s.
-    revert Heqr0. simpl in x.
-    unfold eq_rect in H0.
-    destruct p.
-    unfold desugar_action' in x.
-    unfold RV32I.end_execution in x.
-    simpl in x.
-    unfold x. clear x.
-    intro Heqr0.
-    simpl in Heqr0.
-    apply success_inj in Heqr0.
-    subst.
-    simpl projT1 in v.
-    simpl projT2 in H0.
-
-    inversion H0.
-    apply Eqdep_dec.inj_pair2_eq_dec in H11.
-    2:{
-      apply eq_dec.
-    }
-    apply Eqdep_dec.inj_pair2_eq_dec in H7.
-    apply Eqdep_dec.inj_pair2_eq_dec in H7.
-    apply Eqdep_dec.inj_pair2_eq_dec in H8.
-    apply Eqdep_dec.inj_pair2_eq_dec in H8.
-    apply Eqdep_dec.inj_pair2_eq_dec in H8.
-    assert (var = "res"). eapply EqdepFacts.eq_sigT_fst; eauto. subst.
-    apply Eqdep_dec.inj_pair2_eq_dec in H8.
-    simpl projT1 in *.
-    apply Eqdep_dec.inj_pair2_eq_dec in H10. subst.
-    apply Eqdep_dec.inj_pair2_eq_dec in H.
-    all: try apply eq_dec. clear H0.
-    subst.
-    inv H12.
-    apply Eqdep_dec.inj_pair2_eq_dec in H.
-    apply Eqdep_dec.inj_pair2_eq_dec in H3.
-    apply Eqdep_dec.inj_pair2_eq_dec in H7.
-    apply Eqdep_dec.inj_pair2_eq_dec in H5.
-    apply Eqdep_dec.inj_pair2_eq_dec in H3. subst.
-    all: try apply eq_dec.
-    inv H9.
-    apply Eqdep_dec.inj_pair2_eq_dec in H6.
-    apply Eqdep_dec.inj_pair2_eq_dec in H11.
-    apply Eqdep_dec.inj_pair2_eq_dec in H12.
-    apply Eqdep_dec.inj_pair2_eq_dec in H1.
-    apply Eqdep_dec.inj_pair2_eq_dec in H6. subst.
-    all: try apply eq_dec.
-    inv H8.
-    apply Eqdep_dec.inj_pair2_eq_dec in H4.
-    apply Eqdep_dec.inj_pair2_eq_dec in H9.
-    apply Eqdep_dec.inj_pair2_eq_dec in H9.
-    apply Eqdep_dec.inj_pair2_eq_dec in H9.
-    apply Eqdep_dec.inj_pair2_eq_dec in H12.
-    apply Eqdep_dec.inj_pair2_eq_dec in H14. subst.
-    all: try apply eq_dec.
-
-    apply Eqdep_dec.inj_pair2_eq_dec in H7.
-    apply Eqdep_dec.inj_pair2_eq_dec in H7.
-    apply Eqdep_dec.inj_pair2_eq_dec in H8.
-    apply Eqdep_dec.inj_pair2_eq_dec in H8.
-    apply Eqdep_dec.inj_pair2_eq_dec in H8.
-    assert (var = "res"). eapply EqdepFacts.eq_sigT_fst; eauto. subst.
-    apply Eqdep_dec.inj_pair2_eq_dec in H8.
-    simpl projT1 in *.
-    apply Eqdep_dec.inj_pair2_eq_dec in H10. subst.
-    apply Eqdep_dec.inj_pair2_eq_dec in H.
-    all: try apply eq_dec. clear H0.
-    subst.
-
-    2:{
-      intros. decide equality. apply EqDec_pair.
-    }
-    inversion H11.
-    destruct H11. unfold eq_rect in e.
-    cbn [projT1 projT2] in *.
-
-    vm_compute in H0.
-
-
-    Set Printing Depth 500.
-
-    inv H0.
-
-
-    unfold RV32I.tc_execute in H0.
-    refine (
-      match
-        desugar_action' dummy_pos (fun r : RV32I.reg_t => r)
-        (fun fn => fn) RV32I.execute
-      with
-         x => _
-      end
-    ).
-    fold x in H0.
-    refine ((
-      match
-        TypeInference.tc_action RV32I.R RV32I.Sigma dummy_pos [] unit_t x
-      as r
-      return (
-        TypeInference.tc_action RV32I.R RV32I.Sigma dummy_pos [] unit_t x = r
-        -> is_success r = true -> _
-      ) with
-      | Success s => fun H1 H2 => _
-      | Failure f => fun H1 H2 => _
-      end
-    ) eq_refl eq_refl).
-    2: (simpl in H2; congruence).
-    erewrite extract_success_rewrite in H0. 2: apply H1.
-    simpl (extract_success _ _) in H0.
-    unfold TypeInference.tc_action in H1.
-    destr_in H1. 2: congruence.
-    clear H2.
-    apply cast_action_eq in H1.
-    destruct H1 as (p & EQ). subst s.
-    revert Heqr0. simpl in x.
-    unfold eq_rect in H0.
-    destruct p.
-    unfold desugar_action' in x. cbn in x.
-    unfold x. clear x.
-    intro Heqr0.
-    simpl in Heqr0.
-    vm_compute in Heqr0.
-    apply success_inj in Heqr0.
-
-
-    subst s0. simpl projT1 in v.
-    simpl projT2 in H0.
-    match type of H0 with
-      context [Seq ?a1 ?a2] => set(XX:=a2); fold XX in H0
-    end.
-    inv H0.
-
-    unfold eq_rect in Heqo.
-    destruct p.
-    assert (p = eq_refl).
-    rewrite <- Heqr0 in Heqo.
-    revert H1; rewrite <- Heqr0; clear Heqr0.
-    simpl projT2.
-    intro Hcast; vm_compute in Hcast; inv Hcast.
-
-
-    Heqr0.
-    vm_compute in H1. inv H1. simpl in H2.
-    cbn beta delta iota zeta in H.
-    revert H.
-    unfold opt_bind.
-    destruct may_read.
-    - rewrite H0.
-      rewrite (proj2 (beq_dec_iff _ _ _)). intro A; inv A. reflexivity.
-      reflexivity.
-    - congruence.
-
-    unfold x in H1. vm_compute in H1.
-
-
-
-
-
-    interp_action_t.
+    dependent destruction H.
+    dependent destruction H.
+    dependent destruction H.
+    dependent destruction H.
+    dependent destruction H.
+    dependent destruction H0.
+    destruct (val_eq_dec).
+    rewrite e in H3. contradict H3.
+    unfold l0. simpl. reflexivity.
+    dependent destruction H1.
+    dependent destruction H2. clear H2_.
+    dependent destruction H2_0.
   Qed.
 
   Theorem stack_0_implies_no_setting_halt :
